Liveness.i.dfy
@@ -5,6 +5,7 @@ module Temporal__Liveness_i {
     import opened Temporal__Temporal_s
     import opened Temporal__Lift_i
 
+/*
     // f happens infinitely often.
     // once g happens, it is stable until h
     // f && g ==> h
@@ -27,5 +28,54 @@ module Temporal__Liveness_i {
     {
         // I don't know if this proof rule is actually right. I should
         // probably read the inference rules in Specifying Systems...
+    }
+*/
+
+    lemma InferLeadsTo(f:temporal, g:temporal)
+        requires sat(WF(f))
+        requires sat(until(f, g))
+        ensures sat(leadsto(f, g))
+    {
+        assert sat(always(implies(f, eventually(g))));
+    }
+
+    lemma LeadsToInduction(f:temporal, g:temporal, h:temporal)
+        requires sat(leadsto(f, g));
+        requires sat(leadsto(g, h));
+        ensures sat(leadsto(f, h));
+    {
+        reveal_eventually();
+        assert sat(always(implies(f, eventually(g))));
+
+        forall j | 0 <= j
+            ensures implies(f, eventually(h))(j)
+        {
+            // Unpack the implies
+            if f(j) {
+                // Chain the eventually witnesses together
+                assert implies(f, eventually(g))(j);
+                var k :| j <= k && g(k);
+                assert implies(g, eventually(h))(k);
+            }
+        }
+    }
+
+    lemma AllRoadsLeadTo<T(!new)>(r: QuantifierConstraint<T>,
+        f: QuantifiedTemporal<T>, g: temporal)
+        requires sat(Exists(r, f))
+        requires sat(Forall(r, t => leadsto(f(t), g)))
+        ensures sat(always(eventually(g)))
+    {
+        reveal_eventually();
+        reveal_Exists();
+
+        forall j | 0 <= j
+            ensures eventually(g)(j)
+        {
+            // Find the t that we need at time j to get f(t).
+            var t :| r(t) && f(t)(j);
+            // Then chain f(t) over to eventually-g.
+            assert implies(f(t), eventually(g))(j);
+        }
     }
 }
