simplest-liveness.dfy
@@ -1,0 +1,133 @@
+include "Lift.i.dfy"
+include "Induction.i.dfy"
+include "DafnyPatches.s.dfy"
+include "Liveness.i.dfy"
+
+
+module Jon__simplest_liveness_i {
+import opened Temporal__Temporal_s
+import opened Temporal__Lift_i
+import opened Temporal__Induction_i
+import opened Temporal__Liveness_i
+import opened DafnyPatches_s
+
+function systemSize() : nat // CONSTANT
+    ensures 0 < systemSize()
+    // axiom
+
+datatype System = System(owner:int)
+
+predicate Grant(s:System, s':System) {
+    s'.owner == (s.owner + 1) % systemSize()
+}
+
+predicate Init(s:System) {
+    s.owner == 0
+}
+
+predicate Next(s:System, s':System) {
+    Grant(s, s')
+}
+
+function Spec() : temporal {
+    LiftSpec(Init, Next)
+}
+
+
+predicate Owner(s:System, i:int) {
+    s.owner == i
+}
+
+function OwnerAt(i:int) : StatePredicate<System> {
+    (s:System) => Owner(s, i)
+}
+
+lemma FairnessAxioms()
+    ensures forall i :: 0<=i<systemSize() ==> sat(WF(LiftAction(Grant)))
+// AXIOM
+
+lemma OwnOneHop(i: int)
+    requires sat(Spec())
+    requires 0 <= i < systemSize() - 1
+    ensures sat(leadsto(Lift(OwnerAt(i)), Lift(OwnerAt(i+1))))
+{
+    var f := Lift(OwnerAt(i));
+    var g := Lift(OwnerAt(i+1));
+    InferUntil(Init, Next, OwnerAt(i), OwnerAt(i+1));
+    assert sat(until(f, g));
+    FairnessAxioms();
+    assert sat(WF(f));  // Yeah, how do we get from OwnerAt(i) to LiftAction(Grant)?
+    InferLeadsTo(f, g);
+}
+
+lemma OwnWrap()
+    requires sat(Spec())
+    ensures sat(leadsto(Lift(OwnerAt(systemSize() - 1)), Lift(OwnerAt(0))))
+{
+}
+
+lemma OwnInduction(i: int, j: int)
+    requires sat(Spec())
+    requires 0 <= i < systemSize();
+    requires 0 <= j < systemSize();
+    ensures sat(leadsto(Lift(OwnerAt(i)), Lift(OwnerAt(j))))
+    decreases systemSize() + j - i;
+{
+    if i==j {
+    } else if (i < j) {
+        OwnInduction(i, j-1);
+        OwnOneHop(j-1);
+        LeadsToInduction(Lift(OwnerAt(i)), Lift(OwnerAt(j-1)), Lift(OwnerAt(j)));
+    } else {
+        // i > j: need to wrap.
+        OwnInduction(i, systemSize()-1);
+        OwnWrap();
+        OwnInduction(0, j);
+        LeadsToInduction(Lift(OwnerAt(i)), Lift(OwnerAt(systemSize() - 1)), Lift(OwnerAt(0)));
+        LeadsToInduction(Lift(OwnerAt(i)), Lift(OwnerAt(0)), Lift(OwnerAt(j)));
+    }
+}
+
+lemma OwnForall(j: int)
+    requires sat(Spec())
+    requires 0 <= j < systemSize();
+    //ensures forall i :: 0 <= i < systemSize() ==> sat(leadsto(Lift(OwnerAt(i)), Lift(OwnerAt(j))))
+    ensures sat(Forall(i => 0<=i<systemSize(), i => leadsto(Lift(OwnerAt(i)), Lift(OwnerAt(j)))))
+{
+    forall i | 0 <= i < systemSize()
+        ensures sat(leadsto(Lift(OwnerAt(i)), Lift(OwnerAt(j))))
+    {
+        OwnInduction(i, j);
+    }
+}
+
+lemma AlwaysExistsOwner()
+    requires sat(Spec())
+    ensures sat(Exists(j => 0<=j<systemSize(), j => Lift(OwnerAt(j))))
+{
+}
+
+lemma Liveness()
+    requires sat(Spec())
+    ensures forall j :: 0 <= j < systemSize() ==>
+        sat(always(eventually(Lift(OwnerAt(j)))))
+{
+    forall j | 0 <= j < systemSize()
+        ensures sat(always(eventually(Lift(OwnerAt(j)))))
+    {
+        AlwaysExistsOwner();
+        AllRoadsLeadTo(
+            i => 0 <= i < systemSize(), i => Lift(OwnerAt(i)),
+            Lift(OwnerAt(j)));
+    }
+}
+
+lemma AlwaysEventuallyEveryOwner(i: int)
+    requires sat(Spec())
+    requires 0 <= i < systemSize()
+    ensures sat(always(eventually(Lift(OwnerAt(i)))))
+{
+    // Unpack forall from Liveness?
+}
+
+}
